ADTExamples/QueryStructure/QueryQSSpecs.v
@@ -3,22 +3,30 @@ Require Import List String Ensembles Omega
 
 (* Notations for queries. *)
 
+Definition Query_In (qs : QueryStructureHint) {A} (R : string)
+           (bod : Tuple (schemaHeading
+                           (GetNamedSchema qsSchemaHint R%string)) -> list A) :=
+  fold_right (@app _) (@nil _)
+              (map bod (GetRelation qsHint R%string)).
+
 Notation "( x 'in' R ) bod" :=
-  (fold_right (@app _) nil
-              (map (fun x : Tuple
-                              (schemaHeading
-                                 (GetNamedSchema qsSchemaHint R%string))
-                    => bod)
-                   (GetRelation qsHint R%string))) : QuerySpec_scope.
+  (Query_In _ (R%string) (fun x => bod)) : QuerySpec_scope.
+
+Definition Query_Return {A : Type} (a : A) := (cons a nil).
 
 Notation "'Return' t" :=
-  (cons t%Tuple nil) : QuerySpec_scope.
+  (Query_Return t%Tuple) : QuerySpec_scope.
+
+Definition Query_Where
+           {A : Type} {B B' : Prop} (p : {B} + {B'}) (bod : list A) :=
+  if p%Tuple then bod else nil.
 
 Notation "'Where' p bod" :=
-  (if p%Tuple then bod else nil) : QuerySpec_scope.
+  (Query_Where p%Tuple bod) : QuerySpec_scope.
 
-Notation "'For' bod" := (bod)
-  : QuerySpec_scope.
+Definition Query_For {A} (bod : list A) := bod.
+
+Notation "'For' bod" := (Query_For bod) : QuerySpec_scope.
 
 (* The spec for a count of the number of tuples in a relation. *)
 Definition Count {Schema} (R : list Schema) := List.length R.
